theories/Iris/Model.v
@@ -50,9 +50,10 @@ From Katamaran Require Import
      Syntax.
 Require Import Katamaran.Notation.
 Import ctx.notations.
+Import env.notations.
 
 (* can't import: overlapping notations *)
-Require Katamaran.Sep.Logic.
+Require Import Katamaran.Sep.Logic.
 Module logic := Katamaran.Sep.Logic.
 
 Set Implicit Arguments.
@@ -179,8 +180,6 @@ Module IrisRegisters
        (Import contractkit : SymbolicContractKit termkit progkit assertkit)
        .
 
-  Import EnvNotations.
-
   Module PL := ProgramLogic termkit progkit assertkit contractkit.
   Export PL.
 
@@ -211,8 +210,6 @@ Module Type IrisHeapKit
        (Import assertkit : AssertionKit termkit progkit)
        (Import contractkit : SymbolicContractKit termkit progkit assertkit)
        .
-
-  Import EnvNotations.
 
   Module IrisRegs := IrisRegisters termkit progkit assertkit contractkit.
   Export IrisRegs.
@@ -247,8 +244,6 @@ Module IrisInstance
        (Import assertkit : AssertionKit termkit progkit)
        (Import contractkit : SymbolicContractKit termkit progkit assertkit)
        (Import irisheapkit : IrisHeapKit termkit progkit assertkit contractkit).
-
-  Import EnvNotations.
 
   Section IrisInstance.
 
@@ -433,7 +428,6 @@ Module IrisSoundness
 
   Module Inst := IrisInstance termkit progkit assertkit contractkit irisheapkit.
   Export Inst.
-  Import EnvNotations.
 
   Section IrisSoundness.
 
@@ -651,7 +645,7 @@ Module IrisSoundness
 
   Lemma wp_compat_block {Γ Δ} {τ : Ty} {δ : CStore Γ}
         (δΔ : CStore Δ) (k : Stm (Γ ▻▻ Δ) τ) (Q : Val Γ τ -> iProp Σ) :
-    ⊢ (WP (MkTm (δ ►► δΔ) k) ?{{ v, match v with MkVal _ δ' v => Q (MkVal _ (env_drop Δ δ') v) end }} -∗
+    ⊢ (WP (MkTm (δ ►► δΔ) k) ?{{ v, match v with MkVal _ δ' v => Q (MkVal _ (env.drop Δ δ') v) end }} -∗
           WP (MkTm δ (stm_block δΔ k)) ?{{ v, Q v }})%I.
   Proof.
     iRevert (δ δΔ k Q).
@@ -679,7 +673,7 @@ Module IrisSoundness
       iModIntro.
       dependent elimination H0.
       dependent elimination s; subst δ0.
-      + rewrite env_drop_cat.
+      + rewrite env.drop_cat.
         iFrame.
         iSplitL; [|trivial].
         by iApply wp_value.
@@ -722,7 +716,7 @@ Module IrisSoundness
         (R : Lit τ -> CStore Γ -> iProp Σ) :
         ⊢ (semTriple δ P s Q -∗
                      (∀ (v : Lit σ) (δ' : CStore Γ),
-                         semTriple (env_snoc δ' (x∷σ) v) (Q v δ') k (fun v δ'' => R v (env_tail δ'')) ) -∗
+                         semTriple (env.snoc δ' (x∷σ) v) (Q v δ') k (fun v δ'' => R v (env.tail δ'')) ) -∗
                      semTriple δ P (let: x := s in k) R).
   Proof.
     iIntros "trips tripk P".
@@ -747,7 +741,7 @@ Module IrisSoundness
       iPoseProof ("tripk" $! v _ with "wpv") as "wpk".
       iModIntro.
       iFrame; iSplitL; auto.
-      by iApply (wp_compat_block (env_snoc env_nil (x0∷σ0) v) _ (fun v0 => match v0 with | MkVal _ δ' v1 => R v1 δ' end )).
+      by iApply (wp_compat_block (env.snoc env.nil (x0∷σ0) v) _ (fun v0 => match v0 with | MkVal _ δ' v1 => R v1 δ' end )).
     + iModIntro. iModIntro.
       iMod "Hclose" as "_".
       cbn.
@@ -776,18 +770,18 @@ Module IrisSoundness
         (P : iProp Σ) (Q : Lit σ -> CStore Γ -> iProp Σ)
         (R : Lit τ -> CStore (Γ ▻ x∷σ) -> iProp Σ) :
         ⊢ (semTriple δ P s Q -∗
-                     (∀ (v : Lit σ) (δ' : CStore Γ), semTriple (env_snoc δ' (x∷σ) v) (Q v δ') k R ) -∗
-                     semTriple δ P (let: x := s in k) (fun v δ' => ∃ v__let, R v (env_snoc δ' (x∷σ) v__let)))%I.
+                     (∀ (v : Lit σ) (δ' : CStore Γ), semTriple (env.snoc δ' (x∷σ) v) (Q v δ') k R ) -∗
+                     semTriple δ P (let: x := s in k) (fun v δ' => ∃ v__let, R v (env.snoc δ' (x∷σ) v__let)))%I.
   Proof.
     (* proof should be generalizable beyond Iris model? *)
     iIntros "trips tripk".
-    iApply (iris_rule_stm_let δ s k P Q (fun v δ' => ∃ v__let, R v (env_snoc δ' (x∷σ) v__let))%I with "trips").
+    iApply (iris_rule_stm_let δ s k P Q (fun v δ' => ∃ v__let, R v (env.snoc δ' (x∷σ) v__let))%I with "trips").
     iIntros (v δ') "Qv".
     iPoseProof ("tripk" with "Qv") as "wpk".
     iApply (wp_mono with "wpk").
     iIntros (v') "Rv".
     destruct v'.
-    iExists (env_head δ0).
+    iExists (env.head δ0).
     by dependent elimination δ0.
   Qed.
 
@@ -795,7 +789,7 @@ Module IrisSoundness
         (Δ : PCtx) (δΔ : CStore Δ)
         (τ : Ty) (k : Stm (Γ ▻▻ Δ) τ)
         (P : iProp Σ) (R : Lit τ -> CStore Γ -> iProp Σ) :
-        ⊢ (semTriple (δ ►► δΔ) P k (fun v δ'' => R v (env_drop Δ δ'')) -∗
+        ⊢ (semTriple (δ ►► δΔ) P k (fun v δ'' => R v (env.drop Δ δ'')) -∗
                    semTriple δ P (stm_block δΔ k) R)%I.
   Proof.
     iIntros "tripk P".
@@ -936,7 +930,7 @@ Module IrisSoundness
         (xh xt : 𝑿) (alt_cons : Stm (Γ ▻ xh∷σ ▻ xt∷ty_list σ) τ)
         (P : iProp Σ) (Q : Lit τ -> CStore Γ -> iProp Σ) :
         ⊢ (semTriple δ (P ∧ bi_pure (eval e δ = [])) alt_nil (fun v' δ' => Q v' δ') -∗
-                     (∀ v vs, semTriple (env_snoc (env_snoc δ (xh∷σ) v) (xt∷ty_list σ) vs) (P ∧ bi_pure (eval e δ = cons v vs)) alt_cons (fun v' δ' => Q v' (env_tail (env_tail δ')))) -∗
+                     (∀ v vs, semTriple (env.snoc (env.snoc δ (xh∷σ) v) (xt∷ty_list σ) vs) (P ∧ bi_pure (eval e δ = cons v vs)) alt_cons (fun v' δ' => Q v' (env.tail (env.tail δ')))) -∗
                      semTriple δ P (stm_match_list e alt_nil xh xt alt_cons) Q)%I.
   Proof.
     iIntros "tripnil tripcons P".
@@ -961,7 +955,7 @@ Module IrisSoundness
       iModIntro.
       iFrame.
       iSplitL; [|trivial].
-      iApply (wp_compat_block (env_snoc (env_snoc env_nil (xh0∷σ6) l) (xt0∷ty_list σ6) ls)).
+      iApply (wp_compat_block (env.snoc (env.snoc env.nil (xh0∷σ6) l) (xt0∷ty_list σ6) ls)).
       iApply "tripcons".
       by iFrame.
   Qed.
@@ -972,8 +966,8 @@ Module IrisSoundness
                          (xinr : 𝑿) (alt_inr : Stm (Γ ▻ xinr∷σinr) τ)
                          (P : iProp Σ)
                          (Q : Lit τ -> CStore Γ -> iProp Σ) :
-        ⊢ ((∀ v, semTriple (env_snoc δ (xinl∷σinl) v) (P ∧ ⌜ eval e δ = inl v ⌝) alt_inl (fun v' δ' => Q v' (env_tail δ'))) -∗
-           (∀ v, semTriple (env_snoc δ (xinr∷σinr) v) (P ∧ ⌜ eval e δ = inr v ⌝) alt_inr (fun v' δ' => Q v' (env_tail δ'))) -∗
+        ⊢ ((∀ v, semTriple (env.snoc δ (xinl∷σinl) v) (P ∧ ⌜ eval e δ = inl v ⌝) alt_inl (fun v' δ' => Q v' (env.tail δ'))) -∗
+           (∀ v, semTriple (env.snoc δ (xinr∷σinr) v) (P ∧ ⌜ eval e δ = inr v ⌝) alt_inr (fun v' δ' => Q v' (env.tail δ'))) -∗
         semTriple δ P (stm_match_sum e xinl alt_inl xinr alt_inr) Q)%I.
   Proof.
     iIntros "tripinl tripinr P".
@@ -991,14 +985,14 @@ Module IrisSoundness
       iMod "Hclose" as "_".
       iModIntro. iFrame.
       iSplitL; [|trivial].
-      iApply (wp_compat_block (env_snoc env_nil (xinl0∷σinl0) v1)).
+      iApply (wp_compat_block (env.snoc env.nil (xinl0∷σinl0) v1)).
       iApply ("tripinl" $! v1).
       by iFrame.
     - iModIntro. iModIntro.
       iMod "Hclose" as "_".
       iModIntro. iFrame.
       iSplitL; [|trivial].
-      iApply (wp_compat_block (env_snoc env_nil (xinr0∷σinr0) v2)).
+      iApply (wp_compat_block (env.snoc env.nil (xinr0∷σinr0) v2)).
       iApply ("tripinr" $! v2).
       by iFrame.
   Qed.
@@ -1008,8 +1002,8 @@ Module IrisSoundness
         (xl xr : 𝑿) (rhs : Stm (Γ ▻ xl∷σ1 ▻ xr∷σ2) τ)
         (P : iProp Σ) (Q : Lit τ -> CStore Γ -> iProp Σ) :
         ⊢ ((∀ vl vr,
-            semTriple (env_snoc (env_snoc δ (xl∷σ1) vl) (xr∷σ2) vr)
-              (P ∧ bi_pure (eval e δ = (vl,vr))) rhs (fun v δ' => Q v (env_tail (env_tail δ')))) -∗
+            semTriple (env.snoc (env.snoc δ (xl∷σ1) vl) (xr∷σ2) vr)
+              (P ∧ bi_pure (eval e δ = (vl,vr))) rhs (fun v δ' => Q v (env.tail (env.tail δ')))) -∗
           semTriple δ P (stm_match_prod e xl xr rhs) Q)%I.
   Proof.
     iIntros "trippair P".
@@ -1027,7 +1021,7 @@ Module IrisSoundness
     iMod "Hclose" as "_".
     iModIntro. iFrame.
     iSplitL; [|trivial].
-    iApply (wp_compat_block (env_snoc (env_snoc env_nil (xl0∷σ8) v1) (xr0∷σ9) v2)).
+    iApply (wp_compat_block (env.snoc (env.snoc env.nil (xl0∷σ8) v1) (xr0∷σ9) v2)).
     iApply ("trippair" $! v1 v2).
     by iFrame.
   Qed.
@@ -1059,7 +1053,7 @@ Module IrisSoundness
         {σs : Ctx Ty} {Δ : PCtx} (e : Exp Γ (ty_tuple σs))
         (p : TuplePat σs Δ) {τ : Ty} (rhs : Stm (Γ ▻▻ Δ) τ)
         (P : iProp Σ) (Q : Lit τ -> CStore Γ -> iProp Σ) :
-    ⊢ ((semTriple (env_cat δ (tuple_pattern_match_lit p (eval e δ))) P rhs (fun v δ' => Q v (env_drop Δ δ'))) -∗
+    ⊢ ((semTriple (env.cat δ (tuple_pattern_match_lit p (eval e δ))) P rhs (fun v δ' => Q v (env.drop Δ δ'))) -∗
        semTriple δ P (stm_match_tuple e p rhs) Q)%I.
   Proof.
     iIntros "triptup P".
@@ -1086,7 +1080,7 @@ Module IrisSoundness
         (alt__r : forall (K : 𝑼𝑲 U), Stm (Γ ▻▻ alt__Δ K) τ)
         (P : iProp Σ) (Q : Lit τ -> CStore Γ -> iProp Σ) :
         ⊢ ((∀ (K : 𝑼𝑲 U) (v : Lit (𝑼𝑲_Ty K)),
-               semTriple (env_cat δ (pattern_match_lit (alt__p K) v)) (P ∧ bi_pure (eval e δ = 𝑼_fold (existT K v))) (alt__r K) (fun v δ' => Q v (env_drop (alt__Δ K) δ'))) -∗
+               semTriple (env.cat δ (pattern_match_lit (alt__p K) v)) (P ∧ bi_pure (eval e δ = 𝑼_fold (existT K v))) (alt__r K) (fun v δ' => Q v (env.drop (alt__Δ K) δ'))) -∗
                semTriple δ P (stm_match_union U e alt__p alt__r) Q
           )%I.
   Proof.
@@ -1117,7 +1111,7 @@ Module IrisSoundness
         {R : 𝑹} {Δ : PCtx} (e : Exp Γ (ty_record R))
         (p : RecordPat (𝑹𝑭_Ty R) Δ) {τ : Ty} (rhs : Stm (Γ ▻▻ Δ) τ)
         (P : iProp Σ) (Q : Lit τ -> CStore Γ -> iProp Σ) :
-        ⊢ ((semTriple (env_cat δ (record_pattern_match_lit p (eval e δ))) P rhs (fun v δ' => Q v (env_drop Δ δ'))) -∗
+        ⊢ ((semTriple (env.cat δ (record_pattern_match_lit p (eval e δ))) P rhs (fun v δ' => Q v (env.drop Δ δ'))) -∗
         semTriple δ P (stm_match_record R e p rhs) Q)%I.
   Proof.
     iIntros "triprec P".
@@ -1166,7 +1160,7 @@ Module IrisSoundness
         (x : 𝑿) (σ : Ty) (xIn : x∷σ ∈ Γ) (s : Stm Γ σ)
         (P : iProp Σ) (R : Lit σ -> CStore Γ -> iProp Σ) :
         ⊢ (semTriple δ P s R -∗
-                     semTriple δ P (stm_assign x s) (fun v__new δ' => ∃ v__old, R v__new (@env_update _ _ _ δ' (x∷_)  _ v__old) ∧ bi_pure (env_lookup δ' xIn = v__new)))%I.
+                     semTriple δ P (stm_assign x s) (fun v__new δ' => ∃ v__old, R v__new (@env.update _ _ _ δ' (x∷_)  _ v__old) ∧ bi_pure (env.lookup δ' xIn = v__new)))%I.
   Proof.
     iIntros "trips P".
     iPoseProof ("trips" with "P") as "wpv".
@@ -1192,8 +1186,8 @@ Module IrisSoundness
       iSplitL; [|trivial].
       iApply wp_value.
       cbn.
-      iExists (env_lookup δ1 xInΓ).
-      rewrite env_update_update env_update_lookup env_lookup_update.
+      iExists (env.lookup δ1 xInΓ).
+      rewrite env.update_update env.update_lookup env.lookup_update.
       by iFrame.
     + iModIntro. iModIntro.
       iMod "Hclose" as "_".
@@ -1219,7 +1213,7 @@ Module IrisSoundness
   Lemma iris_rule_stm_assign_backwards {Γ} (δ : CStore Γ)
         (x : 𝑿) (σ : Ty) (xIn : x∷σ ∈ Γ) (s : Stm Γ σ)
         (P : iProp Σ) (R : Lit σ -> CStore Γ -> iProp Σ) :
-        ⊢ (semTriple δ P s (fun v δ' => R v (@env_update _ _ _ δ' (x∷_) _ v)) -∗
+        ⊢ (semTriple δ P s (fun v δ' => R v (@env.update _ _ _ δ' (x∷_) _ v)) -∗
            semTriple δ P (stm_assign x s) R)%I.
   Proof.
     iIntros "trips P".
@@ -1228,7 +1222,7 @@ Module IrisSoundness
     iIntros ([δ' v']) "Rv".
     iDestruct "Rv" as (v__old) "[Rv %]".
     rewrite <-H0.
-    by rewrite env_update_update env_update_lookup.
+    by rewrite env.update_update env.update_lookup.
   Qed.
 
 
@@ -1238,7 +1232,7 @@ Module IrisSoundness
       | Some (MkSepContract _ _ ctxΣ θΔ pre result post) =>
         ∀ (ι : SymInstance ctxΣ),
           semTriple (inst θΔ ι) (interpret_assertion (L:=iProp Σ) pre ι) (Pi f)
-                    (fun v δ' => interpret_assertion post (env_snoc ι (result∷σ) v))
+                    (fun v δ' => interpret_assertion post (env.snoc ι (result∷σ) v))
       | None => True
       end)%I.
 
@@ -1316,7 +1310,7 @@ Module IrisSoundness
     iApply wp_compat_call_frame.
     rewrite H0.
     iApply (wp_mono _ _ _ (fun v => frame ∗ match v with
-                                            | MkVal _ _ v => interpret_assertion ens (env_snoc ι (result∷σ) v)
+                                            | MkVal _ _ v => interpret_assertion ens (env.snoc ι (result∷σ) v)
                                             end)%I).
     - intros [δ' v]; cbn.
       iIntros "[fr ens]".
@@ -1429,7 +1423,7 @@ Module IrisSoundness
         forall (ι : SymInstance Σ'),
         evals es δ = inst θΔ ι ->
         ⊢ semTriple δ (interpret_assertion req ι) (stm_foreign f es)
-          (fun v δ' => interpret_assertion ens (env_snoc ι (result∷τ) v) ∗ bi_pure (δ' = δ))
+          (fun v δ' => interpret_assertion ens (env.snoc ι (result∷τ) v) ∗ bi_pure (δ' = δ))
       end.
 
   Lemma iris_rule_stm_foreign
@@ -1447,7 +1441,7 @@ Module IrisSoundness
     dependent elimination ctrip; cbn in extSem.
     iIntros "P".
     iPoseProof (l with "P") as "[frm pre]".
-    iApply (wp_mono _ _ _ (fun v => frame0 ∗ match v with | MkVal _ δ' v => interpret_assertion ens (env_snoc ι (result∷τ) v) ∗ bi_pure (δ' = δ) end)%I).
+    iApply (wp_mono _ _ _ (fun v => frame0 ∗ match v with | MkVal _ δ' v => interpret_assertion ens (env.snoc ι (result∷τ) v) ∗ bi_pure (δ' = δ) end)%I).
     - intros v.
       destruct v.
       iIntros "[frame [pre %]]".
@@ -1637,8 +1631,6 @@ Module Adequacy
        (Import assertkit : AssertionKit termkit progkit)
        (Import contractkit : SymbolicContractKit termkit progkit assertkit)
        (Import irisheapkit : IrisHeapKit termkit progkit assertkit contractkit).
-
-  Import EnvNotations.
 
   Module PL := ProgramLogic termkit progkit assertkit contractkit.
   Import PL.
