theories/SemiConcrete/Mutator.v
@@ -46,7 +46,7 @@ From Katamaran Require Import
 From stdpp Require base list option.
 
 Import ctx.notations.
-Import EnvNotations.
+Import env.notations.
 Import ListNotations.
 
 Set Implicit Arguments.
@@ -128,7 +128,7 @@ Module SemiConcrete
       forall Δ : NCtx N Ty, CDijkstra (NamedEnv Lit Δ) :=
       fix rec Δ {struct Δ} :=
         match Δ with
-        | ε       => fun k => k env_nil
+        | ε       => fun k => k env.nil
         | Δ ▻ x∷σ => fun k =>
             angelic σ (fun v => rec Δ (fun EΔ => k (EΔ ► (x∷σ ↦ v))))
         end.
@@ -141,7 +141,7 @@ Module SemiConcrete
       forall Δ : NCtx N Ty, CDijkstra (NamedEnv Lit Δ) :=
       fix rec Δ {struct Δ} :=
         match Δ with
-        | ε       => fun k => k env_nil
+        | ε       => fun k => k env.nil
         | Δ ▻ x∷σ => fun k =>
             demonic σ (fun v => rec Δ (fun EΔ => k (EΔ ► (x∷σ ↦ v))))
         end.
@@ -241,14 +241,14 @@ Module SemiConcrete
     Proof.
       induction Δ; cbn.
       - split.
-        + now exists env_nil.
-        + intros [vs ?]. now destruct (nilView vs).
+        + now exists env.nil.
+        + intros [vs ?]. now destruct (env.nilView vs).
       - destruct b as [x σ].
         unfold angelic. split.
         + intros [v Hwp]. apply IHΔ in Hwp.
           destruct Hwp as [vs HPOST].
-          now exists (env_snoc vs (x∷σ) v).
-        + intros [vs Hwp]. destruct (snocView vs) as [vs v].
+          now exists (env.snoc vs (x∷σ) v).
+        + intros [vs Hwp]. destruct (env.snocView vs) as [vs v].
           exists v. apply IHΔ. now exists vs.
     Qed.
 
@@ -258,15 +258,15 @@ Module SemiConcrete
       induction Δ; cbn.
       - split.
         + intros ? vs.
-          now destruct (nilView vs).
+          now destruct (env.nilView vs).
         + now intuition.
       - destruct b as [x σ].
         unfold demonic. split.
         + intros Hwp vs.
-          destruct (snocView vs) as [vs v].
-          now eapply (IHΔ (fun vs => POST (env_snoc vs _ v))).
+          destruct (env.snocView vs) as [vs v].
+          now eapply (IHΔ (fun vs => POST (env.snoc vs _ v))).
         + intros HPost v.
-          now eapply (IHΔ (fun vs => POST (env_snoc vs (x∷σ) v))).
+          now eapply (IHΔ (fun vs => POST (env.snoc vs (x∷σ) v))).
     Qed.
 
     Lemma wp_angelic_list {A} (xs : list A) (POST : A -> Prop) :
@@ -997,10 +997,10 @@ Module SemiConcrete
 
       Definition pushpop {A Γ1 Γ2 x σ} (v : Lit σ)
         (d : CMut (Γ1 ▻ x∷σ) (Γ2 ▻ x∷σ) A) : CMut Γ1 Γ2 A :=
-        fun POST δ0 => d (fun a δ1 => POST a (env_tail δ1)) (δ0 ► (x∷σ ↦ v)).
+        fun POST δ0 => d (fun a δ1 => POST a (env.tail δ1)) (δ0 ► (x∷σ ↦ v)).
       Definition pushspops {A} {Γ1 Γ2 Δ} (δΔ : CStore Δ)
         (d : CMut (Γ1 ▻▻ Δ) (Γ2 ▻▻ Δ) A) : CMut Γ1 Γ2 A :=
-        fun POST δ0 => d (fun a δ1 => POST a (env_drop Δ δ1)) (δ0 ►► δΔ).
+        fun POST δ0 => d (fun a δ1 => POST a (env.drop Δ δ1)) (δ0 ►► δΔ).
       Definition get_local {Γ} : CMut Γ Γ (CStore Γ) :=
         fun POST δ => POST δ δ.
       Definition put_local {Γ1 Γ2} (δ : CStore Γ2) : CMut Γ1 Γ2 unit :=
@@ -1088,8 +1088,8 @@ Module SemiConcrete
         | asn_match_sum σ τ s xl alt_inl xr alt_inr =>
           demonic_match_sum
             (inst (T := fun Σ => Term Σ _) s ι)
-            (fun v => produce (env_snoc ι (xl∷σ) v) alt_inl)
-            (fun v => produce (env_snoc ι (xr∷τ) v) alt_inr)
+            (fun v => produce (env.snoc ι (xl∷σ) v) alt_inl)
+            (fun v => produce (env.snoc ι (xr∷τ) v) alt_inr)
         | asn_match_list s alt_nil xh xt alt_cons =>
           demonic_match_list
             (inst (T := fun Σ => Term Σ _) s ι)
@@ -1117,7 +1117,7 @@ Module SemiConcrete
                          (produce ι a2)
         | asn_exist ς τ a =>
           v <- demonic τ ;;
-          produce (env_snoc ι (ς∷τ) v) a
+          produce (env.snoc ι (ς∷τ) v) a
         | asn_debug => pure tt
         end.
 
@@ -1133,8 +1133,8 @@ Module SemiConcrete
         | asn_match_sum σ τ s xl alt_inl xr alt_inr =>
           angelic_match_sum
             (inst (T := fun Σ => Term Σ _) s ι)
-            (fun v => consume (env_snoc ι (xl∷σ) v) alt_inl)
-            (fun v => consume (env_snoc ι (xr∷τ) v) alt_inr)
+            (fun v => consume (env.snoc ι (xl∷σ) v) alt_inl)
+            (fun v => consume (env.snoc ι (xr∷τ) v) alt_inr)
         | asn_match_list s alt_nil xh xt alt_cons =>
           angelic_match_list
             (inst (T := fun Σ => Term Σ _) s ι)
@@ -1162,7 +1162,7 @@ Module SemiConcrete
                          (consume ι a2)
         | asn_exist ς τ a =>
           v <- angelic τ ;;
-          consume (env_snoc ι (ς∷τ) v) a
+          consume (env.snoc ι (ς∷τ) v) a
         | asn_debug => pure tt
         end.
 
@@ -1177,7 +1177,7 @@ Module SemiConcrete
           assert_formula (inst δ ι = vs) ;;
           consume ι req  ;;
           v <- demonic τ ;;
-          produce (env_snoc ι (result∷τ) v) ens ;;
+          produce (env.snoc ι (result∷τ) v) ens ;;
           pure v
         end.
 
@@ -1260,7 +1260,7 @@ Module SemiConcrete
                 (exec_aux s1)
                 (fun h t =>
                    pushspops
-                     (env_snoc (env_snoc env_nil (xh∷σ) h) (xt∷ty_list σ) t)
+                     (env.snoc (env.snoc env.nil (xh∷σ) h) (xt∷ty_list σ) t)
                      (exec_aux s2))
             | stm_match_sum e xinl s1 xinr s2 =>
               v <- eval_exp e ;;
@@ -1274,7 +1274,7 @@ Module SemiConcrete
                 v
                 (fun vl vr =>
                    pushspops
-                     (env_snoc (env_snoc env_nil (xl∷_) vl) (xr∷_) vr)
+                     (env.snoc (env.snoc env.nil (xl∷_) vl) (xr∷_) vr)
                      (exec_aux s))
             | stm_match_tuple e p rhs =>
               v <- eval_exp e ;;
@@ -1323,7 +1323,7 @@ Module SemiConcrete
           fun ι =>
           produce ι req ;;
           exec inline_fuel s >>= fun v =>
-          consume (env_snoc ι (result∷τ) v) ens
+          consume (env.snoc ι (result∷τ) v) ens
           (* cmut_block *)
           (* cmut_leakcheck *)
         end%mut.
